- Added the two versions of BA to the repository - Some other stuff adding the beginnings of functions - Made a load of rules intro and added some more stuff for alphabets - Proved some more laws in rel

theories/generic/utp_gen_laws.thy
@@ -6,7 +6,7 @@
 header {* Generic Laws *}
 
 theory utp_gen_laws
-imports utp_eval_tactic
+imports utp_eval_tactic "../algebra/alpha_boolean_algebra2"
 begin
 
 context GEN_PRED
@@ -19,5 +19,73 @@ theorem AndP_intro :
 apply (utp_pred_taut_tac)
 apply (auto)
 done
+
+theorem OrP_assoc:
+"\<lbrakk>p1 \<in> WF_ALPHA_PREDICATE;
+ p2 \<in> WF_ALPHA_PREDICATE;
+ p3 \<in> WF_ALPHA_PREDICATE\<rbrakk> \<Longrightarrow>
+ p1 \<or>p (p2 \<or>p p3) = (p1 \<or>p p2) \<or>p p3"
+by (utp_pred_eq_tac) (auto)
+
+theorem OrP_comm:
+"\<lbrakk>p \<in> WF_ALPHA_PREDICATE;
+ q \<in> WF_ALPHA_PREDICATE\<rbrakk> \<Longrightarrow>
+ p \<or>p q = q \<or>p p"
+ by (utp_pred_eq_tac) (auto)
+
+theorem OrP_identity:
+"\<lbrakk> p \<in> WF_ALPHA_PREDICATE;
+   a \<subseteq> \<alpha> p\<rbrakk> \<Longrightarrow>
+ p \<or>p false a = p"
+  apply(frule WF_ALPHA_PREDICATE_subset)
+  apply(auto)
+  apply(utp_pred_eq_tac)
+  apply(auto)
+done
+
+theorem OrP_AndP_dist:
+"\<lbrakk>p1 \<in> WF_ALPHA_PREDICATE;
+ p2 \<in> WF_ALPHA_PREDICATE;
+ p3 \<in> WF_ALPHA_PREDICATE\<rbrakk> \<Longrightarrow>
+ p1 \<or>p (p2 \<and>p p3) = (p1 \<or>p p2) \<and>p (p1 \<or>p p3)"
+apply (utp_pred_eq_tac)
+apply (auto)
+done
+
+theorem huntington:
+ "\<lbrakk>p \<in> WF_ALPHA_PREDICATE;
+   q \<in> WF_ALPHA_PREDICATE;
+   \<alpha> q \<subseteq> \<alpha> p \<rbrakk> \<Longrightarrow>
+  \<not>p (\<not>p p \<or>p \<not>p q) \<or>p \<not>p (\<not>p p \<or>p q) = p"
+  by (utp_pred_eq_tac) (auto)
+
+
+abbreviation "GEN_PRED_algebra \<equiv> \<lparr> alpha_boolean_algebra.carrier = WF_ALPHA_PREDICATE, wfalpha = WF_ALPHABET, alpha = alphabet, conj = AndP, disj = OrP, compl = NotP, top = TrueP, bot = FalseP, ble = (\<lambda> x y. Refinement y x) \<rparr>"
+
 end
+
+sublocale GEN_PRED \<subseteq> alpha_boolean_algebra "GEN_PRED_algebra" where
+"alpha_boolean_algebra.carrier GEN_PRED_algebra = WF_ALPHA_PREDICATE" and
+"wfalpha GEN_PRED_algebra = WF_ALPHABET" and
+"alpha   GEN_PRED_algebra = alphabet" and
+"conj    GEN_PRED_algebra = AndP" and
+"disj    GEN_PRED_algebra = OrP" and
+"compl   GEN_PRED_algebra = NotP"  and
+"top     GEN_PRED_algebra = TrueP" and
+"bot     GEN_PRED_algebra = FalseP" and
+"ble     GEN_PRED_algebra = (\<lambda> x y. Refinement y x)"
+apply(unfold_locales)
+apply(simp_all)
+apply(utp_pred_eq_tac)+
+apply(utp_pred_taut_tac)
+apply(auto)
+apply(erule_tac ballE)+
+apply(auto)
+apply(smt OrP_assoc)
+apply(smt OrP_comm)
+apply(metis OrP_identity set_eq_subset)
+apply(smt OrP_AndP_dist)
+done
+
+
 end
